clean up Graph.v after Smallstep hoist
Removes the now-redundant definitions and lemmas that moved to Smallstep:
inputs_of, output_in_trace, event_guaranteed, allowed_trace, helper lemmas,
and the entire Section node (can/will/sound/complete/monotone/etc.).

Section nodes (1st) now uses Smallstep's can_output/complete_weak/sound/
described_by/monotone' and adds a Local Notation allowed_trace := (allowed_trace A)
so existing proofs keep working.

Section graph (2nd) takes A_graph as an extra Context for the graph-level
allowed predicate (the graph operates at message = node_id * message).

Section graphs is dropped: graphs_sound/complete needed nodes_corresp_* applied
at the graph message type, but nodes_corresp_* is still fixed at Section __'s
message — needs further polymorphism work to lift.

Co-Authored-By: Claude Opus 4.7 <noreply@anthropic.com>

src/datalog/Graph.v
@@ -14,292 +14,59 @@ Section __.
   Context (A : list message -> Prop).
   (*domain is multisets*)
 
+  Local Notation IO_event := (IO_event message).
+
   Section graph.
     Context {node_prog : Type} {graph_prog : map.map node_id node_prog}.
     Context {node_state : Type} {node_states : map.map node_id node_state}.
     Context (p : graph_prog).
 
-    Variant IO_event :=
-      | I_event (_ : message)
-      | O_event (_ : list message).
-
-    Context (node_step : node_prog -> node_state -> IO_event -> node_state -> Prop).
+    Context (node_recv : node_prog -> node_state -> message -> node_state).
+    Context (node_emit : node_prog -> node_state -> list message -> node_state -> Prop).
 
     Record graph_state :=
       { g_nodes : node_states;
         g_messages : list (node_id (*destination*) * message) }.
 
-    Inductive graph_step : graph_state -> IO_event -> graph_state -> Prop :=
-    | gstep_input gs n m :
-      input_allowed n m = true ->
-      graph_step gs (I_event m)
-                 {| g_nodes := gs.(g_nodes);
-                   g_messages := (n, m) :: gs.(g_messages) |}
-    | gstep_run gs n np ns ns' outs :
+    Definition graph_recv (gs : graph_state) (nm : node_id * message) : graph_state :=
+      let '(n, m) := nm in
+      {| g_nodes := gs.(g_nodes);
+        g_messages := (n, m) :: gs.(g_messages) |}.
+
+    Inductive graph_emit : graph_state -> list (node_id * message) -> graph_state -> Prop :=
+    | gemit_run gs n np ns ns' outs :
       map.get p n = Some np ->
       map.get gs.(g_nodes) n = Some ns ->
-      node_step np ns (O_event outs) ns' ->
-      graph_step gs (O_event (filter (output_visible n) outs))
+      node_emit np ns outs ns' ->
+      graph_emit gs (map (fun m => (n, m)) (filter (output_visible n) outs))
                  {| g_nodes := map.put gs.(g_nodes) n ns';
                    g_messages := gs.(g_messages) ++
                                       flat_map (fun m => map (fun n' => (n', m)) (forward n m))
                                       outs |}
-    | gstep_receive gs n np ns ns' m ms1 ms2 :
+    | gemit_receive gs n np ns m ms1 ms2 :
       map.get p n = Some np ->
       map.get gs.(g_nodes) n = Some ns ->
-      node_step np ns (I_event m) ns' ->
       gs.(g_messages) = ms1 ++ (n, m) :: ms2 ->
-      graph_step gs (O_event [])
-                 {| g_nodes := map.put gs.(g_nodes) n ns';
+      graph_emit gs []
+                 {| g_nodes := map.put gs.(g_nodes) n (node_recv np ns m);
                    g_messages := ms1 ++ ms2 |}.
   End graph.
 
-  Definition inputs_of (t : list IO_event) :=
-    flat_map (fun e => match e with I_event m => [m] | _ => [] end) t.
-
-  Definition output_in_trace (output : message) (t : list IO_event) :=
-    exists outs, In (O_event outs) t /\ In output outs.
-
-  Definition event_guaranteed (e : IO_event) :=
-    match e with
-    | O_event _ => True
-    | I_event _ => False
-    end.
-
-  Definition allowed_trace t :=
-    A (inputs_of t).
-
-  Lemma output_in_trace_app o (l1 l2 : list IO_event) :
-    output_in_trace o (l1 ++ l2) <-> output_in_trace o l1 \/ output_in_trace o l2.
-  Proof.
-    unfold output_in_trace; split.
-    - intros (outs & Hin & Hino).
-      apply in_app_or in Hin as [Hin|Hin]; [left|right]; eauto.
-    - intros [(outs & Hin & Hino)|(outs & Hin & Hino)];
-        exists outs; (split; [apply in_or_app|exact Hino]); auto.
-  Qed.
-
-  Lemma output_in_trace_rev o (l : list IO_event) :
-    output_in_trace o (rev l) <-> output_in_trace o l.
-  Proof.
-    unfold output_in_trace; split; intros (outs & Hin & Hino); exists outs;
-      (split; [|exact Hino]); apply in_rev; auto.
-    rewrite rev_involutive. exact Hin.
-  Qed.
-
-  Lemma allowed_trace_universal :
-    (forall t, A t) -> forall t, allowed_trace t.
-  Proof. unfold allowed_trace; auto. Qed.
-
-  Lemma inputs_of_app t1 t2 :
-    inputs_of (t1 ++ t2) = inputs_of t1 ++ inputs_of t2.
-  Proof. apply flat_map_app. Qed.
-
-  Lemma inputs_of_event_guaranteed t :
-    Forall event_guaranteed t -> inputs_of t = [].
-  Proof.
-    induction 1; auto.
-    destruct x; cbn; auto. contradiction.
-  Qed.
-
-  Lemma output_in_trace_swap o l1 e l2 :
-    output_in_trace o (l1 ++ e :: l2) <-> output_in_trace o (e :: l1 ++ l2).
-  Proof.
-    unfold output_in_trace.
-    split; intros (outs & Hin & Hino); exists outs; (split; [|exact Hino]).
-    - apply in_app_or in Hin. destruct Hin as [Hin | [Hin | Hin]].
-      + right. apply in_or_app. left. exact Hin.
-      + left. exact Hin.
-      + right. apply in_or_app. right. exact Hin.
-    - destruct Hin as [Hin | Hin].
-      + apply in_or_app. right. left. exact Hin.
-      + apply in_app_or in Hin. destruct Hin as [Hin | Hin].
-        * apply in_or_app. left. exact Hin.
-        * apply in_or_app. right. right. exact Hin.
-  Qed.
-
-  Section node.
-    Context {node_state : Type}.
-    Context (node_step : node_state -> IO_event -> node_state -> Prop).
-    Context (D : list message (*inputs*) -> message (*output*) -> Prop).
-    Context (initial_ns : node_state).
-
-    Fail Fail Definition node_might_output start t (output : message) : Prop :=
-      exists t' ns,
-        star node_step start t' ns /\
-          allowed_trace (t' ++ t) /\
-          output_in_trace output (t' ++ t).
-
-    Definition node_will_output start t (output : message) : Prop :=
-      eventually (can_step node_step allowed_trace (fun _ => event_guaranteed))
-        (fun '(_, t') => output_in_trace output t')
-        (start, t).
-
-    Definition node_can_output start t output :=
-      exists t' ns,
-        star node_step start t' ns /\
-          Forall event_guaranteed t' /\
-          output_in_trace output (t' ++ t).
-
-    Fail Fail Definition monotone :=
-      forall inputs1 inputs2 output,
-        D inputs1 output ->
-        incl inputs1 inputs2 ->
-        D inputs2 output.
-
-    Definition node_complete :=
-      forall t ns,
-        star node_step initial_ns t ns ->
-        allowed_trace t ->
-        (forall output,
-            D (inputs_of t) output ->
-            node_will_output ns t output).
-
-    Definition node_sound :=
-      forall t ns,
-        star node_step initial_ns t ns ->
-        allowed_trace t ->
-        forall output,
-          output_in_trace output t ->
-          D (inputs_of t) output.
-
-    Definition node_described_by :=
-      node_sound /\ node_complete.
-
-    Fail Fail CoInductive stream {T} :=
-    | scons : T -> stream -> stream.
-    Fail Arguments stream : clear implicits.
-
-    Fail Definition allowed (s : stream IO_event) :=
-        forall o,
-          In o s <-> exists inps, D inps o /\ forall i, In i inps -> In i s.
-
-    (*wrong, since angelic nondeterminism*)
-    Fail Definition node_described_by_omni :=
-      forall s,
-        ~allowed s ->
-        eventually (can_step node_step1 allowed_trace (fun _ => event_guaranteed))
-          (fun '(_, t) => ~prefix t s)
-          (initial_ns, []).
-
-    Definition node_complete_weak :=
-      forall t ns,
-        star node_step initial_ns t ns ->
-        allowed_trace t ->
-        forall output,
-          D (inputs_of t) output ->
-          node_can_output ns t output.
-
-    Definition node_described_by_weak :=
-      node_sound /\ node_complete_weak.
-
-    (*TODO: does having this for each node imply it for the graph?*)
-    (*TODO: this is definitely a property we want to prove about our Datalog nodes.*)
-    Definition can_implies_will :=
-      forall t ns o,
-        star node_step initial_ns t ns ->
-        allowed_trace t ->
-        node_can_output ns t o ->
-        node_will_output ns t o.
-
-    Definition node_monotone :=
-      forall t1 t2 ns1 ns2 o,
-        star node_step initial_ns t1 ns1 ->
-        star node_step ns1 t2 ns2 ->
-        allowed_trace t1 ->
-        allowed_trace (t2 ++ t1) ->
-        node_can_output ns1 t1 o ->
-        node_can_output ns2 (t2 ++ t1) o.
-
-    From Datalog Require Import Tactics.
-    From coqutil Require Import Tactics.fwd.
-
-    Lemma will_implies_can :
-      forall ns t o,
-        allowed_trace t ->
-        node_will_output ns t o ->
-        node_can_output ns t o.
-    Proof.
-      intros ns0 t0 o Hall Hwill.
-      cbv [node_will_output] in Hwill.
-      remember (ns0, t0) as st eqn:Est.
-      revert ns0 t0 Hall Est.
-      induction Hwill as [[ns' t'] HP | [ns' t'] midset Hcan Hmid IH];
-        intros ns0 t0 Hall [= -> ->].
-      - exists [], ns0. split; [constructor|].
-        split; [constructor|exact HP].
-      - cbv [can_step] in Hcan.
-        specialize (Hcan ns0 [] (star_refl _ _)).
-        cbn in Hcan. specialize (Hcan Hall).
-        destruct Hcan as (ns'' & e & Hguar & Hstep & Hmidset).
-        cbn in Hguar.
-        assert (Hall' : allowed_trace (e :: t0)).
-        { unfold allowed_trace; cbn. destruct e; auto. contradiction. }
-        destruct (IH _ Hmidset ns'' (e :: t0) Hall' eq_refl)
-          as (t'' & ns''' & Hstar'' & Hforall'' & Hout'').
-        exists (e :: t''), ns'''.
-        split; [econstructor; eassumption|].
-        split; [constructor; auto|].
-        cbn. apply output_in_trace_swap. exact Hout''.
-    Qed.
-
-    Lemma ciw_monotone :
-      can_implies_will ->
-      node_monotone.
-    Proof.
-      cbv [can_implies_will node_monotone].
-      intros Hciw t1 t2 ns1 ns2 o Hstar1 Hstar2 Hall1 Hallt Hcan.
-      apply (Hciw _ _ _ Hstar1 Hall1) in Hcan.
-      cbv [node_will_output] in Hcan.
-      invert Hcan.
-      - exists [], ns2. split; [constructor|].
-        split; [constructor|].
-        cbn. apply output_in_trace_app. right. exact H.
-      - cbv [can_step] in H.
-        specialize (H _ _ Hstar2 Hallt).
-        destruct H as (ns'' & e & Hguar & Hstep & Hmidset).
-        cbn in Hguar.
-        specialize (H0 _ Hmidset).
-        assert (Hall' : allowed_trace (e :: t2 ++ t1)).
-        { unfold allowed_trace; cbn. destruct e; auto. contradiction. }
-        apply (will_implies_can _ _ _ Hall') in H0.
-        destruct H0 as (t' & ns''' & Hstar' & Hforall' & Hout').
-        exists (e :: t'), ns'''.
-        split; [econstructor; eassumption|].
-        split; [constructor; auto|].
-        cbn. apply output_in_trace_swap. exact Hout'.
-    Qed.
-
-    Definition node_monotone' :=
-      forall t1 t2 ns1 ns2 o,
-        star node_step initial_ns t1 ns1 ->
-        star node_step initial_ns t2 ns2 ->
-        incl (inputs_of t1) (inputs_of t2) ->
-        node_can_output ns1 t1 o ->
-        node_can_output ns2 t2 o.
-
-    (*we want something like this?  idk, anyway we want to find a hypothesis that is
-      the difference node_described_by - can_implies_will.
-      actually, ideally, we want node_described_by - can_implies_will - node_monotone
-     *)
-    Lemma node_complete_weak_implies_strong :
-      node_complete_weak ->
-      can_implies_will ->
-      node_complete.
-    Proof.
-      intros Hweak Hcan t ns Hstar Hall o HD.
-      apply Hcan; auto.
-    Qed.
-  End node.
+  Local Notation allowed_trace := (allowed_trace A).
 
   Section nodes.
     Context {node_state1 : Type}.
-    Context (node_step1 : node_state1 -> IO_event -> node_state1 -> Prop).
+    Context (recv1 : node_state1 -> message -> node_state1).
+    Context (emit1 : node_state1 -> list message -> node_state1 -> Prop).
     Context (initial_ns1 : node_state1).
 
     Context {node_state2 : Type}.
-    Context (node_step2 : node_state2 -> IO_event -> node_state2 -> Prop).
+    Context (recv2 : node_state2 -> message -> node_state2).
+    Context (emit2 : node_state2 -> list message -> node_state2 -> Prop).
     Context (initial_ns2 : node_state2).
+
+    Local Notation node_step1 := (step recv1 emit1).
+    Local Notation node_step2 := (step recv2 emit2).
 
     (*is this just the converse of nodes_corresp_sound?
       yes, obviously---this is why you defined nodes_bicorresp the way it is.
@@ -313,7 +80,7 @@ Section __.
         inputs_of t1 = inputs_of t2 ->
         forall output,
           output_in_trace output t1 ->
-          node_can_output node_step2 ns2 t2 output.
+          can_output node_step2 ns2 t2 output.
 
     Definition nodes_corresp_sound :=
       forall t2 ns2 output,
@@ -326,31 +93,16 @@ Section __.
             output_in_trace output t1.
 
     Lemma complete_sound D :
-      node_complete_weak node_step1 D initial_ns1 ->
+      complete_weak node_step1 A initial_ns1 D ->
       nodes_corresp_complete ->
-      node_complete_weak node_step2 D initial_ns2.
+      complete_weak node_step2 A initial_ns2 D.
     Proof. Abort.
 
     Lemma sound_sound D :
-      node_sound node_step1 D initial_ns1 ->
+      sound node_step1 A initial_ns1 D ->
       nodes_corresp_sound ->
-      node_sound node_step2 D initial_ns2.
+      sound node_step2 A initial_ns2 D.
     Proof. Abort.
-
-    (*no good (eventually is not expressive enough), since angelic nondeterminism*)
-    Fail Fail Definition nodes_corresp_omni :=
-      forall P,
-        eventually (can_step node_step1 allowed_trace (fun _ => event_guaranteed))
-          P (initial_ns1, []) ->
-        eventually (can_step node_step2 allowed_trace (fun _ => event_guaranteed))
-          (fun '(_, t2) =>
-             exists ns1 t1,
-               P (ns1, t1) /\
-                 incl (inputs_of t1) (inputs_of t2) /\
-                 forall o,
-                   output_in_trace o t1 ->
-                   output_in_trace o t2)
-          (initial_ns2, []).
 
     Definition nodes_bicorresp :=
       forall t1 t2 ns1 ns2,
@@ -360,11 +112,11 @@ Section __.
         allowed_trace t2 ->
         inputs_of t1 = inputs_of t2 ->
         forall output,
-          node_can_output node_step1 ns1 t1 output <->
-          node_can_output node_step2 ns2 t2 output.
+          can_output node_step1 ns1 t1 output <->
+          can_output node_step2 ns2 t2 output.
 
     Lemma sound_complete_bicorresp :
-      node_monotone' node_step1 initial_ns1 ->
+      monotone' node_step1 initial_ns1 ->
       nodes_corresp_complete ->
       nodes_corresp_sound ->
       nodes_bicorresp.
@@ -391,7 +143,7 @@ Section __.
           destruct Hout as [Hout|Hout]; [right|left]; exact Hout. }
         destruct (Hsound _ _ _ Hstar2' Hall2' Hout2')
           as (t1' & ns1' & Hstar1' & Heqinp & Hout1).
-        assert (Hcan1' : node_can_output node_step1 ns1' t1' o).
+        assert (Hcan1' : can_output node_step1 ns1' t1' o).
         { exists [], ns1'. split; [constructor|].
           split; [constructor|exact Hout1]. }
         apply (Hmono t1' t1 ns1' ns1 o Hstar1' Hstar1); auto.
@@ -402,27 +154,29 @@ Section __.
     Fail Fail Definition nodes_equiv :=
       exists D,
         (*monotone D /\*)
-        node_described_by node_step1 D initial_ns1 /\
-          node_described_by node_step2 D initial_ns2.
+        described_by node_step1 A initial_ns1 D /\
+          described_by node_step2 A initial_ns2 D.
   End nodes.
 
   Section nodes.
     Context {node_state1 : Type}.
-    Context (node_step1 : node_state1 -> IO_event -> node_state1 -> Prop).
+    Context (recv1 : node_state1 -> message -> node_state1).
+    Context (emit1 : node_state1 -> list message -> node_state1 -> Prop).
     Context (initial_ns1 : node_state1).
 
     Context {node_state2 : Type}.
-    Context (node_step2 : node_state2 -> IO_event -> node_state2 -> Prop).
+    Context (recv2 : node_state2 -> message -> node_state2).
+    Context (emit2 : node_state2 -> list message -> node_state2 -> Prop).
     Context (initial_ns2 : node_state2).
 
     Lemma sound_impl_complete :
-      nodes_corresp_sound node_step1 initial_ns1 node_step2 initial_ns2 ->
-      nodes_corresp_complete node_step2 initial_ns2 node_step1 initial_ns1 .
+      nodes_corresp_sound recv1 emit1 initial_ns1 recv2 emit2 initial_ns2 ->
+      nodes_corresp_complete recv2 emit2 initial_ns2 recv1 emit1 initial_ns1.
     Proof. Abort.
 
     Lemma complete_impl_sound :
-      nodes_corresp_complete node_step2 initial_ns2 node_step1 initial_ns1 ->
-      nodes_corresp_sound node_step1 initial_ns1 node_step2 initial_ns2.
+      nodes_corresp_complete recv2 emit2 initial_ns2 recv1 emit1 initial_ns1 ->
+      nodes_corresp_sound recv1 emit1 initial_ns1 recv2 emit2 initial_ns2.
     Proof. Abort.
 
   End nodes.
@@ -431,52 +185,21 @@ Section __.
     Context {node_prog : Type} {graph_prog : map.map node_id node_prog}.
     Context {node_state : Type} {node_states : map.map node_id node_state}.
     Context (p : graph_prog) (initial_ns : node_states).
-    Context (node_step : node_prog -> node_state -> IO_event -> node_state -> Prop).
+    Context (node_recv : node_prog -> node_state -> message -> node_state).
+    Context (node_emit : node_prog -> node_state -> list message -> node_state -> Prop).
+    Context (A_graph : list (node_id * message) -> Prop).
 
     Definition initial_graph_state : graph_state :=
       {| g_nodes := initial_ns; g_messages := [] |}.
 
     Lemma graph_can_implies_will :
-      Forall2_map (fun _ np ns => can_implies_will (node_step np) ns) p initial_ns ->
-      can_implies_will (graph_step p node_step) initial_graph_state.
+      Forall2_map (fun _ np ns =>
+                     can_implies_will (step (node_recv np) (node_emit np)) A ns) p initial_ns ->
+      can_implies_will (step graph_recv (graph_emit p node_recv node_emit)) A_graph initial_graph_state.
     Proof. Abort.
   End graph.
 
-  Section graphs.
-    Context {node_prog1 : Type} {graph_prog1 : map.map node_id node_prog1}.
-    Context {node_state1 : Type} {node_states1 : map.map node_id node_state1}.
-    Context {node_states1_ok : map.ok node_states1}.
-    Context (p1 : graph_prog1).
-    Context (node_step1 : node_prog1 -> node_state1 -> IO_event -> node_state1 -> Prop).
-    Context (initial_ns1 : node_states1).
-
-    Context {node_prog2 : Type} {graph_prog2 : map.map node_id node_prog2}.
-    Context {node_state2 : Type} {node_states2 : map.map node_id node_state2}.
-    Context {node_states2_ok : map.ok node_states2}.
-    Context (p2 : graph_prog2).
-    Context (node_step2 : node_prog2 -> node_state2 -> IO_event -> node_state2 -> Prop).
-    Context (initial_ns2 : node_states2).
-
-    Theorem graphs_sound :
-      (forall t, A t) ->
-      Forall4_map
-        (fun n np1 np2 ns1 ns2 =>
-           nodes_corresp_sound (node_step1 np1) ns1 (node_step2 np2) ns2)
-        p1 p2 initial_ns1 initial_ns2 ->
-      nodes_corresp_sound (graph_step p1 node_step1) (initial_graph_state initial_ns1) (graph_step p2 node_step2) (initial_graph_state initial_ns2).
-    Proof. Abort.
-
-    Theorem graphs_complete :
-      (forall t, A t) ->
-      Forall4_map
-        (fun n np1 np2 ns1 ns2 =>
-           nodes_corresp_complete (node_step1 np1) ns1 (node_step2 np2) ns2)
-        p1 p2 initial_ns1 initial_ns2 ->
-      nodes_corresp_complete (graph_step p1 node_step1) (initial_graph_state initial_ns1) (graph_step p2 node_step2) (initial_graph_state initial_ns2).
-    Proof. Abort.
-  End graphs.
 End __.
-Arguments IO_event : clear implicits.
 
 Definition translate_event {M M'} (t : M' -> M) (ev : IO_event M') : IO_event M :=
   match ev with
